Lambda/Confluence.lean
@@ -13,7 +13,7 @@ lemma var_reduction {k : Nat} {N : Lambda} : k →βp N ↔ N = k := by
 @[simp]
 lemma abs_reduction {N N' : Lambda} : λ N →βp λ N' ↔ N →βp N' := by
     constructor
-    . intro h; cases h <;> first | rfl | assumption
+    . intro h; cases h; first | rfl | assumption
     . apply BetaP.abs
 
 @[simp]
@@ -29,12 +29,33 @@ lemma betap_appr {N₁ N₂ N' : Lambda} : N₁ →βp N₂ → N'.app N₁ →�
 lemma para_shift_conservation {i j : Nat} {N N' : Lambda} : N →βp N' → (↑) i j N →βp (↑) i j N' := by
     intro h
     induction h generalizing i j with
-    | refl => rfl
+    | var => rfl
     | abs => constructor; aesop
     | app => constructor <;> aesop
     | subst M₁ M₂ N₁ N₂ =>
-        simp_all [beta]
+        simp [beta]
         rw [shift_unshift_swap (Nat.zero_le i) (shifted_subst' 0 M₂ N₂)]
-        simp_all
+        simp
         rw [← shift_shift_swap _ (Nat.zero_le i), ← beta]
         apply BetaP.subst <;> aesop
+
+lemma para_subst' {n} {M N N' : Lambda} : N →βp N' → M[n := N] →βp M[n := N'] := by
+    intros
+    induction M generalizing n N N' with
+    | var => simp; split_ifs; assumption; rfl
+    | app => simp; apply BetaP.app <;> aesop
+    | abs M ih =>
+        simp; apply ih; apply para_shift_conservation; assumption
+
+lemma para_subst {n} {M N M' N' : Lambda} :
+    M →βp M' → N →βp N' → M[n := N] →βp M'[n := N'] := by
+    intro h₁ h₂
+    induction h₁ generalizing n N N' with
+    | var => simp; split_ifs <;> aesop
+    | app => simp; apply BetaP.app <;> aesop
+    | abs _ _ _ ih =>
+        simp; apply ih; apply para_shift_conservation; assumption
+    | subst M M' P P' hm hp ihm ihp =>
+        simp [beta]
+
+        sorry
